@prefix dc:      <http://purl.org/dc/elements/1.1/> .
@prefix rdfs:    <http://www.w3.org/2000/01/rdf-schema#> .
@prefix default:  <http://elfattah.org/ontologies/quran-1.0.owl#> .
@prefix protege:  <http://protege.stanford.edu/plugins/owl/protege#> .
@prefix xsd:     <http://www.w3.org/2001/XMLSchema#> .
@prefix owl:     <http://www.w3.org/2002/07/owl#> .
@prefix rdf:     <http://www.w3.org/1999/02/22-rdf-syntax-ns#> .

default:transliteration
      a       owl:AnnotationProperty , owl:DatatypeProperty ;
      rdfs:comment "Transliteration of arabic text in Internationalized Phonetic Alphabet (IPA)."@en ;
      rdfs:range xsd:string .

default:hasAyat
      a       owl:ObjectProperty ;
      rdfs:subPropertyOf default:hasElement ;
      owl:inverseOf default:isAyatOf .

default:theHolyQuran
      a       default:Quran ;
      rdfs:comment """There can be one and only one Quran individual.

All Quran individuals must be asserted or inferred to be a synonym of this one."""@en ;
      rdfs:isDefinedBy <http://en.wikipedia.org/wiki/Quran> , <http://dbpedia.org/resource/Qur%27an> ;
      dc:contributor ""^^xsd:string .

<http://elfattah.org/ontologies/quran-1.0.owl>
      a       owl:Ontology ;
      rdfs:comment "El-Fattah Quran Verses Ontology"@en ;
      owl:imports <http://protege.stanford.edu/plugins/owl/dc/protege-dc.owl> , <http://protege.stanford.edu/plugins/owl/protege> .

default:isElementOf
      a       owl:TransitiveProperty , owl:ObjectProperty ;
      owl:inverseOf default:hasElement .

default:Sura
      a       owl:Class ;
      rdfs:comment "The Holy Quran contains 114 Suras."^^xsd:string ;
      owl:disjointWith default:Ajza , default:Ayat ;
      owl:equivalentClass
              [ a       owl:Class ;
                owl:intersectionOf ([ a       owl:Restriction ;
                            owl:hasValue default:theHolyQuran ;
                            owl:onProperty default:isSuraOf
                          ] default:AyatContainer)
              ] .

default:Tafsir
      a       owl:Class ;
      owl:equivalentClass
              [ a       owl:Restriction ;
                owl:onProperty default:isTafsirOf ;
                owl:someValuesFrom
                        [ a       owl:Class ;
                          owl:unionOf (default:Element default:Quran)
                        ]
              ] .

default:Ajza
      a       owl:Class ;
      rdfs:comment """Quran is made of 30 Ajza's.

There is a crosscutting division into 30 parts, ajza, each containing two units called ahzab, each of which is divided into four parts (rub 'al-ahzab). The Qur’an is also divided into seven stations (manazil)

The thirty ajza can be used to read through the entire Qur’an in a week or a month. Some of these parts are known by names and these names are the first few words by which the juz' starts. A juz' is sometimes further divided into two ahzab, and each hizb subdivided into four rub 'al-ahzab."""^^xsd:string ;
      rdfs:subClassOf default:AyatContainer ;
      owl:disjointWith default:Sura , default:Ayat .

default:hasTafsir
      a       owl:ObjectProperty ;
      owl:inverseOf default:isTafsirOf .

default:hasAjza
      a       owl:ObjectProperty ;
      rdfs:subPropertyOf default:hasElement ;
      owl:inverseOf default:isAjzaOf .

default:AyatContainer
      a       owl:Class ;
      owl:disjointWith default:Ayat ;
      owl:equivalentClass
              [ a       owl:Class ;
                owl:intersectionOf ([ a       owl:Restriction ;
                            owl:allValuesFrom default:Ayat ;
                            owl:onProperty default:hasAyat
                          ] default:Element [ a       owl:Restriction ;
                            owl:onProperty default:hasAyat ;
                            owl:someValuesFrom default:Ayat
                          ])
              ] .

default:isTafsirOf
      a       owl:ObjectProperty ;
      owl:inverseOf default:hasTafsir .

default:isAyatOf
      a       owl:ObjectProperty ;
      rdfs:subPropertyOf default:isElementOf ;
      owl:inverseOf default:hasAyat .

default:hasElement
      a       owl:TransitiveProperty , owl:ObjectProperty ;
      owl:inverseOf default:isElementOf .

default:isAjzaOf
      a       owl:ObjectProperty ;
      rdfs:subPropertyOf default:isElementOf ;
      owl:inverseOf default:hasAjza .

default:hasSura
      a       owl:ObjectProperty ;
      rdfs:subPropertyOf default:hasElement ;
      owl:inverseOf default:isSuraOf .

default:Ayat
      a       owl:Class ;
      rdfs:comment """A Quran Sura contains one or more ayat (verses).

Each sura is formed from several ayat (verses), which originally means a sign or portent sent by God. The number of ayat differ from sura to sura. An individual ayah may be just a few letters or several lines. The ayat are unlike the highly refined poetry of the pre-Islamic Arabs in their content and distinctive rhymes and rhythms, being more akin to the prophetic utterances marked by inspired discontinuities found in the sacred scriptures of Judaism and Christianity. The actual number of ayat has been a controversial issue among Muslim scholars since Islam's inception, some recognizing 6,000, some 6,204, some 6,219, and some 6,236, although the words in all cases are the same. The most popular edition of the Qur’an, which is based on the Kufa school tradition, contains 6,236 ayat."""^^xsd:string ;
      owl:disjointWith default:AyatContainer , default:Sura , default:Ajza ;
      owl:equivalentClass
              [ a       owl:Class ;
                owl:intersectionOf (default:Element [ a       owl:Restriction ;
                            owl:allValuesFrom default:AyatContainer ;
                            owl:onProperty default:isAyatOf
                          ])
              ] .

default:Quran
      a       owl:Class ;
      rdfs:comment "The class of Quran itself."^^xsd:string ;
      owl:disjointWith default:Element ;
      owl:equivalentClass
              [ a       owl:Class ;
                owl:intersectionOf ([ a       owl:Restriction ;
                            owl:cardinality "114"^^xsd:int ;
                            owl:onProperty default:hasSura ;
                            owl:valuesFrom default:Sura
                          ] [ a       owl:Restriction ;
                            owl:cardinality "30"^^xsd:int ;
                            owl:onProperty default:hasAjza
                          ] [ a       owl:Restriction ;
                            owl:minCardinality "6000"^^xsd:int ;
                            owl:onProperty default:hasAyat
                          ] [ a       owl:Restriction ;
                            owl:maxCardinality "6236"^^xsd:int ;
                            owl:onProperty default:hasAyat
                          ] [ a       owl:Restriction ;
                            owl:allValuesFrom default:Element ;
                            owl:onProperty default:hasElement
                          ] [ a       owl:Restriction ;
                            owl:allValuesFrom default:Sura ;
                            owl:onProperty default:hasSura
                          ] [ a       owl:Restriction ;
                            owl:allValuesFrom default:Ajza ;
                            owl:onProperty default:hasAjza
                          ])
              ] .

default:Element
      a       owl:Class ;
      rdfs:subClassOf owl:Thing ;
      rdfs:subClassOf
              [ a       owl:Restriction ;
                owl:allValuesFrom default:Tafsir ;
                owl:onProperty default:hasTafsir
              ] ;
      owl:disjointWith default:Quran ;
      owl:equivalentClass
              [ a       owl:Restriction ;
                owl:hasValue default:theHolyQuran ;
                owl:onProperty default:isElementOf
              ] .

default:isSuraOf
      a       owl:ObjectProperty ;
      rdfs:subPropertyOf default:isElementOf ;
      owl:inverseOf default:hasSura .
